poSTVM/poSTVM_alt.thy
@@ -1,0 +1,344 @@
+theory poSTVM_alt
+  imports 
+    "~~/poST/poSTVM/poSTVM_state_alt" 
+begin
+datatype statement_result = Break | Continue | Exit | Return | Reset | NextState
+
+text "Executing unary operation"
+definition unary_op_exec :: "unary_op => basic_post_type \<Rightarrow> basic_post_type" where
+"unary_op_exec op var = (case op of unary_op.Not \<Rightarrow> (basic_post_type_not var) | unary_op.Minus \<Rightarrow> (basic_post_type_minus var))"
+
+text "Executing binary operation"
+definition binary_op_exec :: "binary_op \<Rightarrow> basic_post_type \<Rightarrow> basic_post_type \<Rightarrow> basic_post_type" where
+"binary_op_exec op var1 var2 = 
+  (case op of 
+    binary_op.And \<Rightarrow> basic_post_type.Bool(basic_post_type_and var1 var2)|
+ binary_op.Or \<Rightarrow> basic_post_type.Bool(basic_post_type_or var1 var2)|
+    binary_op.Xor \<Rightarrow> basic_post_type.Bool(basic_post_type_xor var1 var2) | 
+    binary_op.Eq \<Rightarrow> basic_post_type.Bool(basic_post_type_or var1 var2)| 
+    binary_op.NotEq \<Rightarrow>basic_post_type.Bool(basic_post_type_noteq var1 var2)| 
+    binary_op.Less \<Rightarrow>basic_post_type.Bool(basic_post_type_less var1 var2)| 
+    binary_op.More \<Rightarrow>basic_post_type.Bool(basic_post_type_more var1 var2)| 
+    binary_op.LessEq \<Rightarrow>basic_post_type.Bool(basic_post_type_lesseq var1 var2)| 
+    binary_op.MoreEq \<Rightarrow>basic_post_type.Bool(basic_post_type_moreeq var1 var2)| 
+    binary_op.Sum \<Rightarrow> basic_post_type_sum var1 var2| 
+    binary_op.Sub \<Rightarrow> basic_post_type_sub var1 var2| 
+    binary_op.Mul \<Rightarrow> basic_post_type_mul var1 var2| 
+    binary_op.Div \<Rightarrow> basic_post_type_div var1 var2| 
+    binary_op.Mod \<Rightarrow> basic_post_type_mod var1 var2)"
+
+function (sequential) skip_expr :: "expr_stack \<Rightarrow> expr_stack" where 
+  "skip_expr [] = []"
+| "skip_expr ((expr_op.Unary _)#other)= skip_expr other"
+| "skip_expr ((expr_op.Binary _)#other)= skip_expr (skip_expr other)"
+| "skip_expr ((expr_op.Value _)#other) = other"
+| "skip_expr ((expr_op.Get _)#other) = other"
+| "skip_expr ((expr_op.GetArray _)#other) = skip_expr other"
+| "skip_expr ((expr_op.CheckProcStat _ _)#other) = other"
+| "skip_expr ((expr_op.FunctionCall _ _)#other) = other"
+  by pat_completeness auto
+
+lemma length_skip_expr [termination_simp]:
+    "skip_expr_dom xs \<Longrightarrow> length (skip_expr xs) \<le> length xs"
+  by (induction xs rule: skip_expr.pinduct) (auto simp: skip_expr.psimps)
+
+termination skip_expr by lexicographic_order
+
+lemma skip_expr_lessening:
+  "length (skip_expr xs) \<le> length xs"
+  by (induction xs rule: skip_expr.induct) auto
+
+lemma shift_skip_expr_lessening:
+  "length (skip_expr (skip_expr xs)) \<le> length (skip_expr xs)"
+  by (induction xs rule: skip_expr.induct) (auto simp add: skip_expr_lessening)
+
+lemma skip_expr_lessening_suc:
+  "length (skip_expr xs) \<le> Suc (length xs)"
+  by (induction xs rule: skip_expr.induct) (auto simp add: skip_expr_lessening)
+
+lemma double_skip_expr_lessening : 
+    "length (skip_expr (skip_expr xs)) \<le> length xs"
+  by (induction xs rule: skip_expr.induct) (auto simp add: skip_expr_lessening  Nat.le_SucI Orderings.preorder_class.order.trans)
+
+fun skip_exprs :: "nat \<Rightarrow> expr_stack \<Rightarrow> expr_stack" where
+  "skip_exprs (Suc n) [] = []"
+| "skip_exprs (Suc n) ((expr_op.Unary _)#other)= skip_exprs (Suc n) other"
+| "skip_exprs (Suc n) ((expr_op.Binary _)#other)= skip_exprs (Suc (Suc n)) other"
+| "skip_exprs (Suc n) ((expr_op.Value _)#other) = skip_exprs n other"
+| "skip_exprs (Suc n) ((expr_op.Get _)#other) = skip_exprs n other"
+| "skip_exprs (Suc n) ((expr_op.GetArray _)#other) = skip_exprs (Suc n) other"
+| "skip_exprs (Suc n) ((expr_op.CheckProcStat _ _)#other) = skip_exprs n other"
+| "skip_exprs (Suc n) ((expr_op.FunctionCall _ _)#other) = skip_exprs n other"
+
+fun get_sev_expr :: "nat \<Rightarrow> expr_stack \<Rightarrow> expr_stack list" where
+  "get_sev_expr 0 _ = []"
+| "get_sev_expr (Suc n) [] = []"
+| "get_sev_expr (Suc n) ((expr_op.Unary unary_op_option)#other) = 
+    (case (get_sev_expr (Suc n) other) of
+    (first#rest) \<Rightarrow> ((expr_op.Unary unary_op_option) # first) # rest)"
+| "get_sev_expr (Suc n) ((expr_op.Binary binary_op)#other) =
+    (case (get_sev_expr (Suc (Suc n)) other) of
+    (first#second#rest) \<Rightarrow> ((expr_op.Binary binary_op) # first @ second) # rest)"
+| "get_sev_expr (Suc n) ((expr_op.Value val)#other) =
+    [expr_op.Value val] # (get_sev_expr n other)"
+| "get_sev_expr (Suc n) ((expr_op.Get val)#other) =
+    [expr_op.Get val] # (get_sev_expr n other)"
+| "get_sev_expr (Suc n) ((expr_op.GetArray val)#other) =
+    (case (get_sev_expr (Suc n) other) of
+    (first#rest) \<Rightarrow> ((expr_op.GetArray val) # first) # rest)"
+| "get_sev_expr (Suc n) ((expr_op.CheckProcStat val1 val2)#other) =
+    [expr_op.CheckProcStat val1 val2] # (get_sev_expr n other)"
+| "get_sev_expr (Suc n) ((expr_op.FunctionCall val1 val2)#other) =
+    [expr_op.FunctionCall val1 val2] # (get_sev_expr n other)"
+
+
+definition get_one_expr :: "expr_stack \<Rightarrow> expr_stack" where 
+  "get_one_expr st = (nth (get_sev_expr 1 st) 0)"
+
+definition get_expr :: "expr_stack \<Rightarrow> expr_stack * expr_stack" where
+"get_expr st = ((get_one_expr st), (skip_expr st))"
+
+text "Unwind stack until end or break point returning stack starting with the following instruction"
+fun skip_after_break :: "statement_stack \<Rightarrow> statement_stack" where
+"skip_after_break [] = []" |
+"skip_after_break ((statement_op.SetPoint point_type.Break)#other) = other" |
+"skip_after_break (_#other) = other"
+
+text "Unwind stack until end or exit point returning stack starting with the following instruction"
+fun skip_after_exit :: "statement_stack \<Rightarrow> statement_stack" where
+"skip_after_exit [] = []" |
+"skip_after_exit ((statement_op.SetPoint point_type.Exit)#other) = other" |
+"skip_after_exit (_#other) = other"
+
+text "Unwind stack until end or return point returning stack starting with the following instruction"
+fun skip_after_return :: "statement_stack \<Rightarrow> statement_stack" where
+"skip_after_return [] = []" |
+"skip_after_return ((statement_op.SetPoint point_type.Return)#other) = other" |
+"skip_after_return (_#other) = other"
+
+text "Skipping statement list instruction if it next"
+fun skip_statement_list :: "statement_stack \<Rightarrow> statement_stack" where
+"skip_statement_list [] = []" |
+"skip_statement_list ((statement_op.StatementList loc_stack)#other) = other" |
+"skip_statement_list other = other"
+
+text "Converting stack Values to list of basic values. Assuming stack has only Value operationss"
+fun values_to_basics :: "expr_stack \<Rightarrow> basic_post_type list" where
+  "values_to_basics [] = []" 
+| "values_to_basics ((expr_op.Value val)#other) = val # (values_to_basics other)" 
+| "values_to_basics other = [] "
+
+fun get_cases :: "statement_stack \<Rightarrow> statement_stack * statement_stack" where
+  "get_cases [] = ([],[])"
+| "get_cases ((statement_op.CaseStatement nat_list)#(statement_op.StatementList st_list)#other) =
+    (let (cases,rest) = get_cases other
+      in ((statement_op.CaseStatement nat_list)#(statement_op.StatementList st_list)#cases,rest))"
+| "get_cases other = ([],other)"
+
+text "Checking if value contains in list of values "
+primrec contains_basic :: "nat list \<Rightarrow> basic_post_type \<Rightarrow> bool" where
+"contains_basic [] _ = False" |
+"contains_basic (val1#other) val2 = 
+  (if (basic_post_type_eq (basic_post_type.Nat val1) val2) 
+    then True
+    else (contains_basic other val2))"
+
+fun exec_sev_expr :: "nat \<Rightarrow> expr_stack \<Rightarrow> model_state \<Rightarrow> (basic_post_type option) list" where
+  "exec_sev_expr 0 _ st = [None]"
+| "exec_sev_expr (Suc n) [] st = [None]"
+| "exec_sev_expr (Suc n) ((expr_op.Unary unary_op_option)#other) st = 
+  (case (unary_op_option,(exec_sev_expr (Suc n) other st)) of
+    (None,(first#rest)) \<Rightarrow> (first#rest) 
+  | (Some un_op,(first#rest)) \<Rightarrow> ((Some (unary_op_exec un_op (the first)))# rest))"
+| "exec_sev_expr (Suc n) ((expr_op.Binary bin_op)#other) st =
+  (case (exec_sev_expr (Suc (Suc n)) other st) 
+    of (first#second#rest) \<Rightarrow> (Some (binary_op_exec bin_op (the first) (the second)))#rest)"
+| "exec_sev_expr (Suc n) ((expr_op.Value val)#other) st = 
+    (Some val)#(exec_sev_expr n other st)"
+| "exec_sev_expr (Suc n) ((expr_op.Get var_name)#other) st = 
+ (Some (get_symbvar_by_name st var_name))#(exec_sev_expr n other st) " 
+
+| "exec_sev_expr (Suc n) ((expr_op.GetArray var_name) #other) st =
+  (case (exec_sev_expr (Suc n) other st)
+    of (first#rest) \<Rightarrow> (Some (get_arvar_by_name st var_name (the first)))#rest )" 
+
+| "exec_sev_expr (Suc n) ((expr_op.CheckProcStat proc_name proc_stat)#other) st = 
+  (Some (check_proc_status st proc_name proc_stat))#(exec_sev_expr n other st)" 
+(*TO DO Function Call*)
+| "exec_sev_expr (Suc n) ((expr_op.FunctionCall v1 v2)#other) st  =
+  None#(exec_sev_expr n other st)" 
+
+fun exec_expr :: "expr_stack \<Rightarrow> model_state \<Rightarrow> basic_post_type option" where
+ "exec_expr st model_st = nth (exec_sev_expr 1 st model_st) 0"
+
+text "Initialization of array"
+fun initialize_array :: "model_state \<Rightarrow> stacked_var_init \<Rightarrow> stacked_var_init" where
+"initialize_array st var= 
+  (case var of 
+    (stacked_var_init.Array interval values (Some expr_list)) \<Rightarrow> 
+      (stacked_var_init.Array
+        (case interval of
+          (stacked_array_interval.Expr exp1 exp2) \<Rightarrow> 
+            (stacked_array_interval.Int (basic_post_type_to_int (the (exec_expr exp1 st))) (basic_post_type_to_int (the (exec_expr exp2 st)))) |
+          (stacked_array_interval.Int int1 int2) =>
+            (stacked_array_interval.Int int1 int2))
+        (map 
+          (\<lambda>exp. (the (exec_expr exp st)))
+          expr_list)
+        None) |
+    (stacked_var_init.Array interval values None) \<Rightarrow> 
+      (stacked_var_init.Array 
+        (case interval of
+          (stacked_array_interval.Expr exp1 exp2) \<Rightarrow> 
+            (stacked_array_interval.Int (basic_post_type_to_int (the (exec_expr exp1 st))) (basic_post_type_to_int (the (exec_expr exp2 st)))) |
+          (stacked_array_interval.Int int1 int2) =>
+            (stacked_array_interval.Int int1 int2)) 
+        values 
+        None))"
+
+text "Initialization of symbolic variable"
+fun initialize_symbolic :: "model_state \<Rightarrow> stacked_var_init  \<Rightarrow> stacked_var_init" where
+"initialize_symbolic st var= 
+  (case var of
+    (stacked_var_init.Symbolic value (Some init_stack)) \<Rightarrow> 
+      (stacked_var_init.Symbolic (the (exec_expr init_stack st)) None) |
+    (stacked_var_init.Symbolic value None) \<Rightarrow> 
+      (stacked_var_init.Symbolic value None))"
+
+(*TO DO FunctionBlock init*)
+text "Initialization of stacked var"
+fun initialize_stacked_vars :: "model_state \<Rightarrow> stacked_vars \<Rightarrow> stacked_vars" where
+"initialize_stacked_vars st vars =
+  (fmmap
+    (\<lambda>init.
+      (case init of
+        (stacked_var_init.Symbolic value init_option) \<Rightarrow> (initialize_symbolic st init) |
+        (stacked_var_init.Array interval values init_option) \<Rightarrow> (initialize_array st init) |
+        (stacked_var_init.FunctionBlock name) \<Rightarrow> (stacked_var_init.FunctionBlock name)) )
+    vars) "
+
+text "Initialization of proc_vars"
+fun initialize_stacked_proc_vars :: "model_state \<Rightarrow> stacked_proc_var list \<Rightarrow> stacked_proc_var list" where
+"initialize_stacked_proc_vars _ [] = []" |
+"initialize_stacked_proc_vars st (proc_var#other) = 
+  ((case proc_var of
+    (stacked_proc_var.Var stacked_vars) \<Rightarrow> (stacked_proc_var.Var (initialize_stacked_vars st stacked_vars))|
+    (stacked_proc_var.ProcessVar var) \<Rightarrow> (stacked_proc_var.ProcessVar var)|
+    (stacked_proc_var.InOutVar stacked_vars) \<Rightarrow> (stacked_proc_var.InOutVar (initialize_stacked_vars st stacked_vars)) |
+    (stacked_proc_var.InVar stacked_vars) \<Rightarrow> (stacked_proc_var.InVar (initialize_stacked_vars st stacked_vars))|
+    (stacked_proc_var.OutVar stacked_vars) \<Rightarrow> (stacked_proc_var.OutVar (initialize_stacked_vars st stacked_vars)))
+  #(initialize_stacked_proc_vars st other))"
+
+(*TO DO*)
+text "Initialization of process variables"
+fun initialize_process_vars :: "model_state \<Rightarrow> model_state" where
+"initialize_process_vars (model_state.ST global_vars_list (program_map,cur_prog_name) fb_decl_list f_decl_list) =
+  (let st = (model_state.ST global_vars_list (program_map,cur_prog_name) fb_decl_list f_decl_list) 
+  in  (model_state.ST 
+    global_vars_list 
+    (fmmap 
+       (\<lambda>(var_list,proc_map,proc_name). 
+          (var_list,
+            (fmmap 
+              (\<lambda>(var_list,v1,v2,v3,v4).
+                (initialize_stacked_proc_vars st var_list,v1,v2,v3,v4))
+              proc_map),
+          proc_name)) 
+       program_map,
+      cur_prog_name) 
+    fb_decl_list 
+    f_decl_list))"
+
+text "Initialization of prog_vars"
+fun initialize_stacked_prog_vars :: "model_state \<Rightarrow> stacked_prog_var list \<Rightarrow> stacked_prog_var list" where
+"initialize_stacked_prog_vars _ [] = []" |
+"initialize_stacked_prog_vars st (prog_var#other) = 
+  ((case prog_var of
+    (stacked_prog_var.ExtVar stacked_vars) \<Rightarrow> (stacked_prog_var.ExtVar (initialize_stacked_vars st stacked_vars))|
+    (stacked_prog_var.Var stacked_vars) \<Rightarrow> (stacked_prog_var.Var (initialize_stacked_vars st stacked_vars))|
+    (stacked_prog_var.InOutVar stacked_vars) \<Rightarrow> (stacked_prog_var.InOutVar (initialize_stacked_vars st stacked_vars))|
+    (stacked_prog_var.InVar stacked_vars) \<Rightarrow> (stacked_prog_var.InVar (initialize_stacked_vars st stacked_vars))|
+    (stacked_prog_var.OutVar stacked_vars) \<Rightarrow> (stacked_prog_var.OutVar (initialize_stacked_vars st stacked_vars)))
+   #(initialize_stacked_prog_vars st other))"
+
+(*TO DO*)
+text "Initialization of program variables"
+fun initialize_program_vars :: "model_state \<Rightarrow> model_state" where
+"initialize_program_vars (model_state.ST global_vars_list (program_map,cur_prog_name) fb_decl_list f_decl_list) =
+  (let st = (model_state.ST global_vars_list (program_map,cur_prog_name) fb_decl_list f_decl_list)
+  in (model_state.ST 
+    global_vars_list 
+    (fmmap 
+       (\<lambda>(var_list,proc_map,proc_name). 
+          (initialize_stacked_prog_vars st var_list,proc_map,proc_name)) 
+       program_map,
+      cur_prog_name) 
+    fb_decl_list 
+    f_decl_list))"
+
+(*statement_result = Break | Continue | Exit | Return | Reset | NextState*)
+
+primrec get_first_imp_res :: "statement_result list \<Rightarrow> statement_result" where
+  "get_first_imp_res [] = statement_result.Continue"
+| "get_first_imp_res (st_res#other) = 
+  (case st_res of
+    (statement_result.Continue) \<Rightarrow> (get_first_imp_res other)
+  | (statement_result.Return) \<Rightarrow> (statement_result.Return)
+  | (statement_result.Exit) \<Rightarrow> (statement_result.Exit)
+  | (statement_result.Break) \<Rightarrow> (statement_result.Break)
+  | (statement_result.Reset) \<Rightarrow> (statement_result.Reset)
+  | (statement_result.NextState) \<Rightarrow> (statement_result.NextState))"
+
+definition unpack_bool :: "basic_post_type \<Rightarrow> bool" where
+  "unpack_bool val = (case val of (basic_post_type.Bool val) \<Rightarrow> val)"
+
+fun exec_sev_statements :: "nat \<Rightarrow> statement_stack \<Rightarrow> model_state \<Rightarrow> model_state * statement_result" where
+  "exec_sev_statements 0 _ st = (st, statement_result.Continue)"
+| "exec_sev_statements (Suc n) [] st = (st,statement_result.Return)"
+| "exec_sev_statements (Suc n) ((statement_op.Assign var_name exp)#other) st =
+    (exec_sev_statements n other 
+      (set_symbvar st var_name 
+        (the (exec_expr exp st))))"
+| "exec_sev_statements (Suc n) ((statement_op.AssignArray var_name exp)#other) st =
+     (let (pos_stack,new_stack1) = (get_expr exp);
+          (val_stack,_) = (get_expr new_stack1);
+          new_st = (set_arvar st var_name (the (exec_expr pos_stack st)) (the (exec_expr val_stack st)))
+        in (exec_sev_statements n other new_st))"
+(*TO DO FunctionBlockCall 
+| "exec_sev_statements (Suc n) ((stack_op.FunctionBlockCall fb_name param_assign_list )#other) st = "
+*)
+| "exec_sev_statements (Suc n) ((statement_op.SetPoint p)#other) st = (exec_sev_statements n other st)"
+| "exec_sev_statements (Suc n) ((statement_op.GoPoint p)#other) st = 
+    (case p of 
+      point_type.Break \<Rightarrow> (st, statement_result.Break)
+    | point_type.Exit \<Rightarrow>  (st, statement_result.Exit)
+    | point_type.Return \<Rightarrow>  (st, statement_result.Return))"
+| "exec_sev_statements (Suc n) ((statement_op.SetState state_name_option)#other) st =
+    (case state_name_option of
+    None \<Rightarrow> (st, statement_result.NextState) |
+    (Some st_name) \<Rightarrow> (set_state st st_name, statement_result.Return))"
+| "exec_sev_statements (Suc n) ((statement_op.ProcessStatement proc_name_option proc_mod)#other) st =
+  (case proc_name_option of
+    None \<Rightarrow> 
+      (case proc_mod of
+        (process_mod.Restart) \<Rightarrow> (reset_same_process st, statement_result.Return)
+      | (process_mod.Stop) \<Rightarrow> (stop_same_process st, statement_result.Return)
+      | (process_mod.Error) \<Rightarrow> (error_same_process st, statement_result.Return))
+  | (Some proc_name) \<Rightarrow> 
+      (exec_sev_statements n other
+        (case proc_mod of
+          (process_mod.Restart) \<Rightarrow> (reset_process st proc_name)
+        | (process_mod.Stop) \<Rightarrow> (stop_process st proc_name)
+        | (process_mod.Error) \<Rightarrow> (error_process st proc_name))))"
+| "exec_sev_statements (Suc n) ((statement_op.IfStatement exp)#(statement_op.StatementList st_stack)#other) st =
+      (if (unpack_bool (the (exec_expr exp st))) 
+        then 
+          (let (new_st,st_result) = (exec_sev_statements (length st_stack) st_stack st)
+              in (case st_result of
+                    (statement_result.Break) => (exec_sev_statements n (skip_after_break other) new_st)
+                  | (_) \<Rightarrow> (new_st,st_result)))
+        else 
+          (exec_sev_statements n other st))"
+
+
+end
